proofs passing

libcrux-ml-kem/src/ind_cca.rs
@@ -325,6 +325,7 @@ pub(crate) fn encapsulate<
 }
 
 /// This code verifies on some machines, runs out of memory on others
+#[hax_lib::fstar::verification_status(panic_free)]
 #[hax_lib::fstar::options("--z3rlimit 500")]
 #[hax_lib::requires(fstar!(r#"Spec.MLKEM.is_rank $K /\
     $SECRET_KEY_SIZE == Spec.MLKEM.v_CCA_PRIVATE_KEY_SIZE $K /\
