libcrux-ml-kem/proofs/fstar/extraction/Libcrux_ml_kem.Polynomial.fsti
@@ -106,8 +106,8 @@ val to_i16_array
       (out: t_Slice i16)
     : Prims.Pure (t_Slice i16)
       (requires
-        (v_VECTORS_IN_RING_ELEMENT *! mk_usize 16 <: usize) <=.
-        (Core.Slice.impl__len #i16 out <: usize))
+        (Core.Slice.impl__len #i16 out <: usize) >=.
+        (v_VECTORS_IN_RING_ELEMENT *! mk_usize 16 <: usize))
       (fun _ -> Prims.l_True)
 
 val from_bytes
@@ -202,21 +202,6 @@ val impl_2__ZERO:
     Prims.unit
   -> Prims.Pure (t_PolynomialRingElement v_Vector) Prims.l_True (fun _ -> Prims.l_True)
 
-/// Size of a ring element in bytes.
-val impl_2__num_bytes:
-    #v_Vector: Type0 ->
-    {| i1: Libcrux_ml_kem.Vector.Traits.t_Operations v_Vector |} ->
-    Prims.unit
-  -> Prims.Pure usize Prims.l_True (fun _ -> Prims.l_True)
-
-/// The length of a vector of ring elements in bytes
-val vec_len_bytes:
-    v_K: usize ->
-    #v_Vector: Type0 ->
-    {| i1: Libcrux_ml_kem.Vector.Traits.t_Operations v_Vector |} ->
-    Prims.unit
-  -> Prims.Pure usize Prims.l_True (fun _ -> Prims.l_True)
-
 /// Given two polynomial ring elements `lhs` and `rhs`, compute the pointwise
 /// sum of their constituent coefficients.
 val impl_2__add_to_ring_element
@@ -262,6 +247,26 @@ val impl_2__ntt_multiply
       (self rhs: t_PolynomialRingElement v_Vector)
     : Prims.Pure (t_PolynomialRingElement v_Vector) Prims.l_True (fun _ -> Prims.l_True)
 
+/// Size of a ring element in bytes.
+val impl_2__num_bytes:
+    #v_Vector: Type0 ->
+    {| i1: Libcrux_ml_kem.Vector.Traits.t_Operations v_Vector |} ->
+    Prims.unit
+  -> Prims.Pure usize
+      Prims.l_True
+      (ensures
+        fun result ->
+          let result:usize = result in
+          result =. mk_usize 512)
+
+/// The length of a vector of ring elements in bytes
+val vec_len_bytes:
+    v_K: usize ->
+    #v_Vector: Type0 ->
+    {| i1: Libcrux_ml_kem.Vector.Traits.t_Operations v_Vector |} ->
+    Prims.unit
+  -> Prims.Pure usize (requires v_K <=. mk_usize 4) (fun _ -> Prims.l_True)
+
 val impl_2__from_i16_array
       (#v_Vector: Type0)
       {| i1: Libcrux_ml_kem.Vector.Traits.t_Operations v_Vector |}
@@ -299,7 +304,15 @@ val vec_from_bytes
       {| i1: Libcrux_ml_kem.Vector.Traits.t_Operations v_Vector |}
       (bytes: t_Slice u8)
       (out: t_Slice (t_PolynomialRingElement v_Vector))
-    : Prims.Pure (t_Slice (t_PolynomialRingElement v_Vector)) Prims.l_True (fun _ -> Prims.l_True)
+    : Prims.Pure (t_Slice (t_PolynomialRingElement v_Vector))
+      (requires
+        (Core.Slice.impl__len #(t_PolynomialRingElement v_Vector) out <: usize) <=. mk_usize 4 &&
+        (((v_VECTORS_IN_RING_ELEMENT *! mk_usize 16 <: usize) *! mk_usize 2 <: usize) *!
+          (Core.Slice.impl__len #(t_PolynomialRingElement v_Vector) out <: usize)
+          <:
+          usize) <=.
+        (Core.Slice.impl__len #u8 bytes <: usize))
+      (fun _ -> Prims.l_True)
 
 val impl_2__to_bytes
       (#v_Vector: Type0)
@@ -320,6 +333,10 @@ val vec_to_bytes
       (out: t_Slice u8)
     : Prims.Pure (t_Slice u8)
       (requires
-        ((v_VECTORS_IN_RING_ELEMENT *! mk_usize 16 <: usize) *! mk_usize 2 <: usize) <=.
+        (Core.Slice.impl__len #(t_PolynomialRingElement v_Vector) re <: usize) <=. mk_usize 4 &&
+        (((v_VECTORS_IN_RING_ELEMENT *! mk_usize 16 <: usize) *! mk_usize 2 <: usize) *!
+          (Core.Slice.impl__len #(t_PolynomialRingElement v_Vector) re <: usize)
+          <:
+          usize) <=.
         (Core.Slice.impl__len #u8 out <: usize))
       (fun _ -> Prims.l_True)
